theories/PCP/Reductions/PCPb_iff_dPCPb.v
@@ -3,33 +3,14 @@ Import ListNotations.
 
 Require Import Undecidability.PCP.PCP.
 Require Import Undecidability.PCP.Util.Facts.
+Require Import Undecidability.PCP.Reductions.PCPX_iff_dPCP.
 
 Require Import Undecidability.Problems.Reduction.
 
 Require Import Undecidability.Shared.Prelim.
 
-Lemma derivable_BPCP X (P : stack X) u v :
-  derivable P u v -> exists A, incl A P /\ A <> nil /\ tau1 A = u /\ tau2 A = v.
-Proof.
-  induction 1 as [ | ? ? ? ? ? ? (A & ? & ? & ? & ?)].
-  - exists [(x, y)]. repeat split; cbn; simpl_list; eauto. congruence.
-  - subst. exists ((x, y) :: A). repeat split. eauto. congruence.
-Qed.
-    
-Lemma BPCP_derivable X (P : stack X) u v : (exists A, A <<= P /\ A <> nil /\ tau1 A = u /\ tau2 A = v) -> derivable P u v.
-Proof.
-  intros (A & ? & ? & ? & ?). subst. 
-  revert H. pattern A. revert A H0. eapply list_ind_ne; cbn; intros; destruct x as (x,y).
-  - simpl_list. eauto using der_sing, der_cons.
-  - eauto using der_sing, der_cons.
-Qed.
-
 Lemma PCPb_iff_dPCPb P : PCPb P <-> dPCPb P.
-Proof.
-  split.
-  - intros (? & ? & ? & ?). econstructor. eapply BPCP_derivable. eauto.
-  - intros []. edestruct (derivable_BPCP H) as (? & ? & ? & ? & ?). subst. exists x0. eauto.
-Qed.
+Proof. apply PCPX_iff_dPCP. Qed.
 
 Lemma reductionLR : PCPb ⪯ dPCPb.
 Proof.
@@ -38,5 +19,5 @@ Qed.
 
 Lemma reductionRL : dPCPb ⪯ PCPb.
 Proof.
-  exists id. intro x. now rewrite PCPb_iff_dPCPb.
+  exists id. intro. now rewrite PCPb_iff_dPCPb.
 Qed.
